Introduce separate Terminates/Goes_wrong traces (I)
Split stopped finite traces and full finite prefixes into two: the
already existing [tstop] will stand for normal termination, whereas the
newly introduced [tstuck] now represents an abnormal termination. This
brings the trace model closer to that of, say, CompCert.

Up to this point, no changes go beyond straightforward adjustments.
Coming to single continuations, however, we will need to modify the
statements and see how these will affect other results further down.

TraceModel.v
@@ -9,6 +9,7 @@ Require Import List.
 (** *traces  *)
 CoInductive trace : Set :=
   | tstop : trace
+  | tstuck : trace
   | tsilent : trace
   | tcons : event -> trace -> trace.
 
@@ -17,14 +18,15 @@ Definition pref := list event.
 
 Inductive finpref : Set :=
 | fstop : pref -> finpref
+| fstuck : pref -> finpref
 | ftbd  : pref -> finpref
 .
 
 Tactic Notation "destruct" "finpref" ident(m) "as" ident(e) ident(p) :=
-  destruct m as [[|e p] | [|e p]].
+  destruct m as [[| |e p] | [| |e p]].
 
 Tactic Notation "induction" "finpref" ident(m) "as" ident(e) ident(p) ident(Hp) :=
-  destruct m as [m | m]; induction m as [|e p Hp].
+  destruct m as [m | m | m]; induction m as [|e p Hp].
 
 (** *prefix relation *)
 Fixpoint fstop_prefix (m : pref) (t : trace) : Prop :=
@@ -32,6 +34,14 @@ Fixpoint fstop_prefix (m : pref) (t : trace) : Prop :=
     | nil, tstop => True
     | nil, _     => False
     | cons e1 m', tcons e2 t' => e1 = e2 /\ fstop_prefix m' t'
+    | _, _       => False
+  end.
+
+Fixpoint fstuck_prefix (m : pref) (t : trace) : Prop :=
+  match m, t with
+    | nil, tstuck => True
+    | nil, _     => False
+    | cons e1 m', tcons e2 t' => e1 = e2 /\ fstuck_prefix m' t'
     | _, _       => False
   end.
 
@@ -45,6 +55,7 @@ Fixpoint ftbd_prefix (m : pref) (t : trace) : Prop :=
 Definition prefix (m : finpref) (t : trace) : Prop :=
   match m with
   | fstop m => fstop_prefix m t    
+  | fstuck m => fstuck_prefix m t
   | ftbd m  => ftbd_prefix m t
   end.
 
@@ -54,6 +65,7 @@ Definition prefix (m : finpref) (t : trace) : Prop :=
    Eventually they may be given more memorable names than term/nonterm. *)
 Inductive fin : trace -> Prop :=
   | fin_stop : fin tstop
+  | fin_stuck : fin tstuck
   | fin_cons : forall e t, fin t -> fin (tcons e t).
 
 Definition inf (t : trace) : Prop := ~(fin t).
@@ -77,7 +89,20 @@ Proof.
   induction finpref m as e m IHm; intros ta Hinf.
   + exists tstop. split; try now auto.
     intros Hc; subst. apply Hinf. now constructor.
-  + destruct ta as [| | e' ta].
+  + destruct ta as [| | | e' ta].
+    ++ exfalso. apply Hinf. now constructor.
+    ++ exfalso. apply Hinf. now constructor.
+    ++ specialize (IHm tsilent Hinf).
+       destruct IHm as [t' [Hpref Hnsilent]].
+       exists (tcons e t'). now split.
+    ++ apply inf_tcons in Hinf. specialize (IHm ta Hinf).
+       destruct IHm as [t' [Hpref Hneq]]. exists (tcons e t').
+       split; try now auto.
+       intros Hc. inversion Hc; now subst.
+  + exists tstuck. split; try now auto.
+    intros Hc; subst. apply Hinf. now constructor.
+  + destruct ta as [| | | e' ta].
+    ++ exfalso. apply Hinf. now constructor.
     ++ exfalso. apply Hinf. now constructor.
     ++ specialize (IHm tsilent Hinf).
        destruct IHm as [t' [Hpref Hnsilent]].
@@ -88,7 +113,8 @@ Proof.
        intros Hc. inversion Hc; now subst.
   + exists tstop. split; try now auto.
     intros Hc; subst. apply Hinf. now constructor.
-  + destruct ta as [| | e' ta].
+  + destruct ta as [| | | e' ta].
+    ++ exfalso. apply Hinf. now constructor.
     ++ exfalso. apply Hinf. now constructor.
     ++ specialize (IHm tsilent Hinf).
        destruct IHm as [t' [Hpref Hnsilent]].
@@ -108,11 +134,19 @@ Fixpoint fstop_equal (m : pref) (t : trace) : Prop :=
   | _, _ => False
   end.
 
+Fixpoint fstuck_equal (m : pref) (t : trace) : Prop :=
+  match m, t with
+  | nil, tstuck => True
+  | cons e1 m', tcons e2 t' => e1 = e2 /\ fstuck_equal m' t'
+  | _, _ => False
+  end.
+
 Definition ftbd_equal (m : pref) (t : trace) : Prop := False.
 
 Definition equal (m : finpref) (t : trace) : Prop :=
   match m with
   | fstop m => fstop_equal m t
+  | fstuck m => fstuck_equal m t
   | ftbd m  => ftbd_equal m t
   end.
 
@@ -124,21 +158,28 @@ Qed.
 Lemma fin_equal : forall t, fin t <-> exists m : finpref, equal m t.
 Proof.
   intro t. split.
-  - intro H. induction H as [| e t H [m IH]].
-    now (exists (fstop nil)). destruct m as [m | m].
-    now (exists (fstop (cons e m))).
-    now simpl in IH.                         
+  - intro H. induction H as [| | e t H [m IH]].
+    + now (exists (fstop nil)).
+    + now (exists (fstuck nil)).
+    + destruct m as [m | m | m].
+      * now (exists (fstop (cons e m))).
+      * now (exists (fstuck (cons e m))).
+      * now simpl in IH.
   - intros [m Heq]. generalize dependent t.
     induction finpref m as e m' IH; intros t Heq; try now auto.
     + destruct t; try now auto. now constructor.
-    + destruct t as [| | e' t']; inversion Heq.
+    + destruct t as [| | | e' t']; inversion Heq.
+      constructor. now apply IH.
+    + destruct t as [| | | e' t']; inversion Heq.
+      now constructor.
+    + destruct t as [| | | e' t']; inversion Heq.
       constructor. now apply IH.
 Qed.
 
 Lemma single_cont : forall m t t', equal m t -> prefix m t' -> t = t'.
 Proof.
-  induction finpref m as e p IHp; destruct t, t'; firstorder.
-  subst. now rewrite (IHp t t').
+  induction finpref m as e p IHp; destruct t, t'; firstorder;
+  subst; now rewrite (IHp t t').
 Qed.
 
 Lemma single_cont_consequence : forall t,
@@ -161,7 +202,7 @@ Lemma stop_sngle_continuation : forall m t1 t2,
     prefix m t1 -> prefix m t2 ->
     t1 = t2.
 Proof.
-  intros [m | m]; induction m; intros [] [] H H0 H1; try now auto.
+  intros [m | m | m]; induction m; intros [] [] H H0 H1; try now auto.
   + inversion H0. inversion H1. clear H0 H1.
     subst. simpl in H. specialize (IHm t t0 H H3 H5).
     now subst.
